Add Conv_Oom. Prove conversion and GEP cases for concretize_err_fin_inf.

src/coq/Semantics/DynamicValues.v
@@ -2905,9 +2905,10 @@ Module DVALUE(A:Vellvm.Semantics.MemoryAddress.ADDRESS)(IP:Vellvm.Semantics.Memo
       with only four cases to actually build the tree.
      *)
     Variant conv_case : Set :=
-    | Conv_Pure (x : dvalue)
-    | Conv_ItoP (x : dvalue)
-    | Conv_PtoI (x : dvalue)
+    | Conv_Pure    (x : dvalue)
+    | Conv_ItoP    (x : dvalue)
+    | Conv_PtoI    (x : dvalue)
+    | Conv_Oom     (s: string)
     | Conv_Illegal (s: string).
 
     Variant ptr_conv_cases : Set :=
